Automata/Demos.lean
@@ -5,12 +5,13 @@ import Automata.Projection
 
 theorem zero_is_zero : 0 = 0 := by
   apply (eqBase_iff_equal 2 (by norm_num) [0, 0] 2 (by norm_num) 0 1).mpr
-  rfl
+  unfold DFAO.eval DFAO.evalFrom
+  native_decide
+
 
 theorem foo : 100000 = 100000 := by
   apply (eqBase_iff_equal 2 (by norm_num) [100000, 100000] 2 (by norm_num) 0 1).mpr
   native_decide
-
 
 -- What's difficult
 -- ∃ x, x = 0?
@@ -21,3 +22,5 @@ theorem foo : 100000 = 100000 := by
 -- Wrong! Why? Projection only searches for representations in restricted length, 1+1 = 2 needs 2 bits.
 #eval (project 2 (addBase 2)).eval [fun _ => 0, fun _ => 1]
 -- Correct after padding with 0s
+
+#eval (project 2 (addBase 2)).fixLeadingZeros.eval [fun _ => 1]
