Automata/Projection.lean
@@ -8,7 +8,6 @@ import Automata.Pumping
 import Automata.Input
 import Automata.LeadingZeros
 import Automata.Fin
-import Automata.Collapse
 
 def project (m : Fin (n+1)) (dfa : DFA (Fin (n+1) → Fin (b+2)) state) [DecidableEq state] :
   NFA (Fin n → Fin (b+2)) state := {
@@ -80,7 +79,7 @@ theorem project_transFrom [DecidableEq state](dfa : DFA (Fin (n + 1) → Fin (b+
   induction l generalizing states
   case nil =>
     simp only [NFA.transFrom, List.mem_singleton] at h
-    simp_all only [List.nil_eq, List.map_eq_nil, exists_eq_left]
+    simp_all only [List.nil_eq, List.map_eq_nil_iff, exists_eq_left]
     use q
     simp only [h, DFAO.transFrom, and_self]
   case cons f fs ih =>
@@ -184,70 +183,70 @@ theorem project_fix_respectZero [Fintype state][DecidableEq state] (dfa : DFA (F
     . use (Fintype.card (ListND state) + k)
     . exact h'
 
-theorem list_project_aux (x b : ℕ) (l : List ℕ) (hl : l.length = len)(m : Fin (len + 1)) : reverseInput (List.map (fun f ↦ remove_index m f) (inputToBase (b + 2) (by norm_num) (List.insertNth m x l) (by
-      simp_rw[← hl]
-      apply List.length_insertNth
-      omega
-    ))) = l := by
-  sorry
+-- theorem list_project_aux (x b : ℕ) (l : List ℕ) (hl : l.length = len)(m : Fin (len + 1)) : reverseInput (List.map (fun f ↦ remove_index m f) (inputToBase (b + 2) (by norm_num) (List.insertNth m x l) (by
+--       simp_rw[← hl]
+--       apply List.length_insertNth
+--       omega
+--     ))) = l := by
+--   sorry
 
-theorem list_project (x b : ℕ) (l : List ℕ) (hl : l.length = len)(m : Fin (len + 1)) : ∃ k, (List.map (fun f ↦ remove_index m f) (inputToBase (b + 2) (by norm_num) (List.insertNth m x l) (by
-      simp_rw[← hl]
-      apply List.length_insertNth
-      omega
-    ))) = padZeros k (inputToBase (b+2) (by norm_num) l (by omega)) := by
+-- theorem list_project (x b : ℕ) (l : List ℕ) (hl : l.length = len)(m : Fin (len + 1)) : ∃ k, (List.map (fun f ↦ remove_index m f) (inputToBase (b + 2) (by norm_num) (List.insertNth m x l) (by
+--       simp_rw[← hl]
+--       apply List.length_insertNth
+--       omega
+--     ))) = padZeros k (inputToBase (b+2) (by norm_num) l (by omega)) := by
 
-  have := inputToBase_of_reverseInput (List.map (fun f ↦ remove_index m f) (inputToBase (b + 2) (by norm_num) (List.insertNth m x l) (by
-      simp_rw[← hl]
-      apply List.length_insertNth
-      omega
-    )))
-  rcases this with ⟨k, h⟩
-  use k
-  rw[h]
-  congr
-  exact list_project_aux x b l hl m
+--   have := inputToBase_of_reverseInput (List.map (fun f ↦ remove_index m f) (inputToBase (b + 2) (by norm_num) (List.insertNth m x l) (by
+--       simp_rw[← hl]
+--       apply List.length_insertNth
+--       omega
+--     )))
+--   rcases this with ⟨k, h⟩
+--   use k
+--   rw[h]
+--   congr
+--   exact list_project_aux x b l hl m
 
-theorem correct_project [Fintype state] [DecidableEq state] (l : List ℕ) (hl : l.length = len)(m : Fin (len + 1)) (dfa : DFA (Fin (len+1) → Fin (b+2)) state) (hres: dfa.respectZero):
-  (∃ (x : ℕ), dfa.eval (inputToBase (b+2) (by norm_num) (l.insertNth m x) (by simp_rw[← hl]; apply List.length_insertNth; omega))) → (project m dfa).fixLeadingZeros.eval (inputToBase (b+2) (by omega) l hl):= by
-  rw[NFA.fixLeadingZeros_eval]
-  intro h
-  rcases h with ⟨x, h⟩
-  have := eval_project dfa m (inputToBase (b+2) (by norm_num) (l.insertNth m x) (by simp_rw[← hl]; apply List.length_insertNth; omega)) h
-  have lis := list_project x b l hl m
-  rcases lis with ⟨k, h₁⟩
-  rw[h₁] at this
-  apply (project m dfa).bounded_accept _
-  . apply project_acceptZero
-    exact DFA.acceptZero_of_respectZero dfa hres
-  swap
-  . exact padZeros k (inputToBase (b+2) (by norm_num) l (by omega))
-  . constructor
-    . use k
-    . exact this
+-- theorem correct_project [Fintype state] [DecidableEq state] (l : List ℕ) (hl : l.length = len)(m : Fin (len + 1)) (dfa : DFA (Fin (len+1) → Fin (b+2)) state) (hres: dfa.respectZero):
+--   (∃ (x : ℕ), dfa.eval (inputToBase (b+2) (by norm_num) (l.insertNth m x) (by simp_rw[← hl]; apply List.length_insertNth; omega))) → (project m dfa).fixLeadingZeros.eval (inputToBase (b+2) (by omega) l hl):= by
+--   rw[NFA.fixLeadingZeros_eval]
+--   intro h
+--   rcases h with ⟨x, h⟩
+--   have := eval_project dfa m (inputToBase (b+2) (by norm_num) (l.insertNth m x) (by simp_rw[← hl]; apply List.length_insertNth; omega)) h
+--   have lis := list_project x b l hl m
+--   rcases lis with ⟨k, h₁⟩
+--   rw[h₁] at this
+--   apply (project m dfa).bounded_accept _
+--   . apply project_acceptZero
+--     exact DFA.acceptZero_of_respectZero dfa hres
+--   swap
+--   . exact padZeros k (inputToBase (b+2) (by norm_num) l (by omega))
+--   . constructor
+--     . use k
+--     . exact this
 
-theorem project_correct [Fintype state] [DecidableEq state] (l : List ℕ) (hl : l.length = len)(m : Fin (len + 1)) (dfa : DFA (Fin (len+1) → Fin (b+2)) state) (hres: dfa.respectZero):
-  (project m dfa).fixLeadingZeros.eval (inputToBase (b+2) (by omega) l hl) → (∃ (x : ℕ), dfa.eval (inputToBase (b+2) (by norm_num) (l.insertNth m x) (by simp_rw[← hl]; apply List.length_insertNth; omega))):= by
+-- theorem project_correct [Fintype state] [DecidableEq state] (l : List ℕ) (hl : l.length = len)(m : Fin (len + 1)) (dfa : DFA (Fin (len+1) → Fin (b+2)) state) (hres: dfa.respectZero):
+--   (project m dfa).fixLeadingZeros.eval (inputToBase (b+2) (by omega) l hl) → (∃ (x : ℕ), dfa.eval (inputToBase (b+2) (by norm_num) (l.insertNth m x) (by simp_rw[← hl]; apply List.length_insertNth; omega))):= by
 
-  intro h
-  rw[NFA.fixLeadingZeros_eval] at h
-  rw[project_eval_iff] at h
-  rcases h with ⟨l₁, hlis, hdfa⟩
-  have : dfa.eval (inputToBase (b + 2) (by norm_num) (reverseInput l₁) (by exact reverseInput_length l₁)) := by
-    have := inputToBase_of_reverseInput l₁
-    rcases this with ⟨k, h⟩
-    rw[h] at hdfa
-    rw[DFA.respectZero] at hres
+--   intro h
+--   rw[NFA.fixLeadingZeros_eval] at h
+--   rw[project_eval_iff] at h
+--   rcases h with ⟨l₁, hlis, hdfa⟩
+--   have : dfa.eval (inputToBase (b + 2) (by norm_num) (reverseInput l₁) (by exact reverseInput_length l₁)) := by
+--     have := inputToBase_of_reverseInput l₁
+--     rcases this with ⟨k, h⟩
+--     rw[h] at hdfa
+--     rw[DFA.respectZero] at hres
 
-    specialize hres (inputToBase (b + 2) (by norm_num) (reverseInput l₁) (by exact reverseInput_length l₁)) k
-    apply hres.mpr
-    exact hdfa
-  use (reverseInput l₁)[m]'(by have := reverseInput_length l₁; omega)
-  have h₁ : (List.insertNth (↑m) ((reverseInput l₁)[m]'(by have := reverseInput_length l₁; omega)) l) = reverseInput l₁ := by
+--     specialize hres (inputToBase (b + 2) (by norm_num) (reverseInput l₁) (by exact reverseInput_length l₁)) k
+--     apply hres.mpr
+--     exact hdfa
+--   use (reverseInput l₁)[m]'(by have := reverseInput_length l₁; omega)
+--   have h₁ : (List.insertNth (↑m) ((reverseInput l₁)[m]'(by have := reverseInput_length l₁; omega)) l) = reverseInput l₁ := by
 
-    sorry
-  simp_rw[h₁]
-  exact this
+--     sorry
+--   simp_rw[h₁]
+--   exact this
 
 
 
